Network_Security_Policy_Verification/TopoS_withOffendingFlows.thy
@@ -17,14 +17,14 @@ context SecurityInvariant_withOffendingFlows
 begin
   text{*We define the monotonicity of @{text "sinvar"}:
   
-  @{term "(\<And> nP N E' E. valid_graph \<lparr> nodes = N, edges = E \<rparr>  \<Longrightarrow> E' \<subseteq> E \<Longrightarrow> sinvar \<lparr> nodes = N, edges = E \<rparr> nP \<Longrightarrow> sinvar \<lparr> nodes = N, edges = E' \<rparr> nP )"}
+  @{term "(\<And> nP N E' E. wf_graph \<lparr> nodes = N, edges = E \<rparr>  \<Longrightarrow> E' \<subseteq> E \<Longrightarrow> sinvar \<lparr> nodes = N, edges = E \<rparr> nP \<Longrightarrow> sinvar \<lparr> nodes = N, edges = E' \<rparr> nP )"}
   
   Having a valid invariant, removing edges retains the validity. I.e.\ prohibiting more, is more or equally secure.
   *}
 
   definition sinvar_mono :: "bool" where
     "sinvar_mono \<longleftrightarrow> (\<forall> nP N E' E. 
-      valid_graph \<lparr> nodes = N, edges = E \<rparr> \<and> 
+      wf_graph \<lparr> nodes = N, edges = E \<rparr> \<and> 
       E' \<subseteq> E \<and> 
       sinvar \<lparr> nodes = N, edges = E \<rparr> nP \<longrightarrow> sinvar \<lparr> nodes = N, edges = E' \<rparr> nP )"
 
@@ -42,7 +42,7 @@ begin
   lemma sinvar_mono_I_proofrule:
   "\<lbrakk> (\<forall> nP (G:: 'v graph). sinvar G nP = (\<forall> (e1, e2) \<in> edges G. P e1 e2 nP G) ); 
     (\<forall> nP e1 e2 N E' E. 
-      valid_graph \<lparr> nodes = N, edges = E \<rparr> \<and> 
+      wf_graph \<lparr> nodes = N, edges = E \<rparr> \<and> 
       (e1,e2) \<in> E \<and> 
       E' \<subseteq> E \<and> 
       P e1 e2 nP \<lparr>nodes = N, edges = E\<rparr> \<longrightarrow> P e1 e2 nP \<lparr>nodes = N, edges = E'\<rparr>) \<rbrakk> \<Longrightarrow> sinvar_mono"
@@ -50,18 +50,18 @@ begin
   proof(clarify)
     fix nP N E' E
     assume AllForm: "(\<forall> nP (G:: 'v graph). sinvar G nP = (\<forall> (e1, e2) \<in> edges G. P e1 e2 nP G) )"
-    and Pmono: "\<forall>nP e1 e2 N E' E. valid_graph \<lparr> nodes = N, edges = E \<rparr> \<and> (e1,e2) \<in> E \<and> E' \<subseteq> E \<and> P e1 e2 nP \<lparr>nodes = N, edges = E\<rparr> \<longrightarrow> P e1 e2 nP \<lparr>nodes = N, edges = E'\<rparr>"
-    and validG: "valid_graph \<lparr>nodes = N, edges = E\<rparr>"
+    and Pmono: "\<forall>nP e1 e2 N E' E. wf_graph \<lparr> nodes = N, edges = E \<rparr> \<and> (e1,e2) \<in> E \<and> E' \<subseteq> E \<and> P e1 e2 nP \<lparr>nodes = N, edges = E\<rparr> \<longrightarrow> P e1 e2 nP \<lparr>nodes = N, edges = E'\<rparr>"
+    and wfG: "wf_graph \<lparr>nodes = N, edges = E\<rparr>"
     and E'subset: "E' \<subseteq> E"
     and evalE: "sinvar \<lparr>nodes = N, edges = E\<rparr> nP"
     
     from Pmono have Pmono1: 
-      "\<And>nP N E' E. valid_graph \<lparr> nodes = N, edges = E \<rparr> \<Longrightarrow> E' \<subseteq> E \<Longrightarrow> (\<forall>(e1,e2) \<in> E. P e1 e2 nP \<lparr>nodes = N, edges = E\<rparr> \<longrightarrow> P e1 e2 nP \<lparr>nodes = N, edges = E'\<rparr>)" 
+      "\<And>nP N E' E. wf_graph \<lparr> nodes = N, edges = E \<rparr> \<Longrightarrow> E' \<subseteq> E \<Longrightarrow> (\<forall>(e1,e2) \<in> E. P e1 e2 nP \<lparr>nodes = N, edges = E\<rparr> \<longrightarrow> P e1 e2 nP \<lparr>nodes = N, edges = E'\<rparr>)" 
     by blast
 
     from AllForm have "sinvar \<lparr>nodes = N, edges = E\<rparr> nP = (\<forall> (e1, e2) \<in> E. P e1 e2 nP \<lparr>nodes = N, edges = E\<rparr>)" by force
     from this evalE have "(\<forall> (e1, e2) \<in> E. P e1 e2 nP \<lparr>nodes = N, edges = E\<rparr>)" by simp
-    from Pmono1[OF validG E'subset, of "nP"] this have "\<forall>(e1, e2) \<in> E. P e1 e2 nP \<lparr>nodes = N, edges = E'\<rparr>" by fast
+    from Pmono1[OF wfG E'subset, of "nP"] this have "\<forall>(e1, e2) \<in> E. P e1 e2 nP \<lparr>nodes = N, edges = E'\<rparr>" by fast
     from this E'subset have "\<forall>(e1, e2) \<in> E'. P e1 e2 nP \<lparr>nodes = N, edges = E'\<rparr>" by fast
     from this have "\<forall>(e1, e2) \<in> (edges \<lparr>nodes = N, edges = E'\<rparr>). P e1 e2 nP \<lparr>nodes = N, edges = E'\<rparr>" by simp
     from this AllForm show "sinvar \<lparr>nodes = N, edges = E'\<rparr> nP" by presburger
@@ -70,16 +70,16 @@ begin
 
    text{*Invariant violations do not disappear if we add more flows. *}
    lemma sinvar_mono_imp_negative_mono:
-   "sinvar_mono \<Longrightarrow> valid_graph \<lparr> nodes = N, edges = E \<rparr> \<Longrightarrow>  E' \<subseteq> E \<Longrightarrow> \<not> sinvar \<lparr> nodes = N, edges = E' \<rparr> nP \<Longrightarrow> \<not> sinvar \<lparr> nodes = N, edges = E \<rparr> nP"
+   "sinvar_mono \<Longrightarrow> wf_graph \<lparr> nodes = N, edges = E \<rparr> \<Longrightarrow>  E' \<subseteq> E \<Longrightarrow> \<not> sinvar \<lparr> nodes = N, edges = E' \<rparr> nP \<Longrightarrow> \<not> sinvar \<lparr> nodes = N, edges = E \<rparr> nP"
    apply (unfold sinvar_mono_def)
    by(blast)
 
   corollary sinvar_mono_imp_negative_delete_edge_mono:
-   "sinvar_mono \<Longrightarrow> valid_graph G \<Longrightarrow> X \<subseteq> Y \<Longrightarrow> \<not> sinvar (delete_edges G Y) nP \<Longrightarrow> \<not> sinvar (delete_edges G X) nP "
+   "sinvar_mono \<Longrightarrow> wf_graph G \<Longrightarrow> X \<subseteq> Y \<Longrightarrow> \<not> sinvar (delete_edges G Y) nP \<Longrightarrow> \<not> sinvar (delete_edges G X) nP "
   proof -
    assume sinvar_mono
-   and "valid_graph G" and "X \<subseteq> Y" and "\<not> sinvar (delete_edges G Y) nP"
-   from delete_edges_valid[OF `valid_graph G`] have valid_G_delete: "valid_graph \<lparr>nodes = nodes G, edges = edges G - X\<rparr>" by(simp add: delete_edges_simp2)
+   and "wf_graph G" and "X \<subseteq> Y" and "\<not> sinvar (delete_edges G Y) nP"
+   from delete_edges_wf[OF `wf_graph G`] have valid_G_delete: "wf_graph \<lparr>nodes = nodes G, edges = edges G - X\<rparr>" by(simp add: delete_edges_simp2)
    from `X \<subseteq> Y` have "edges G - Y \<subseteq> edges G - X" by blast
    with `sinvar_mono` sinvar_mono_def valid_G_delete have
     "sinvar \<lparr>nodes = nodes G, edges = edges G - X\<rparr> nP \<Longrightarrow> sinvar \<lparr>nodes = nodes G, edges = edges G - Y\<rparr> nP" by blast
@@ -103,24 +103,24 @@ begin
   (*use this to show locale preliminaries from mono*)
   lemma sinvar_mono_imp_is_offending_flows_mono:
   assumes mono: "sinvar_mono"
-  and validG: "valid_graph G"
+  and wfG: "wf_graph G"
   shows "is_offending_flows FF G nP  \<Longrightarrow> is_offending_flows (FF \<union> F) G nP"
   proof -
-    from validG have validG': "valid_graph \<lparr>nodes = nodes G, edges = {(e1, e2). (e1, e2) \<in> edges G \<and> (e1, e2) \<notin> FF}\<rparr>" 
-      by (metis delete_edges_def delete_edges_valid)
-    from mono have sinvarE: "(\<And> nP N E' E. valid_graph \<lparr> nodes = N, edges = E \<rparr> \<Longrightarrow> E' \<subseteq> E \<Longrightarrow> sinvar \<lparr> nodes = N, edges = E \<rparr> nP \<Longrightarrow> sinvar \<lparr> nodes = N, edges = E' \<rparr> nP )"
+    from wfG have wfG': "wf_graph \<lparr>nodes = nodes G, edges = {(e1, e2). (e1, e2) \<in> edges G \<and> (e1, e2) \<notin> FF}\<rparr>" 
+      by (metis delete_edges_def delete_edges_wf)
+    from mono have sinvarE: "(\<And> nP N E' E. wf_graph \<lparr> nodes = N, edges = E \<rparr> \<Longrightarrow> E' \<subseteq> E \<Longrightarrow> sinvar \<lparr> nodes = N, edges = E \<rparr> nP \<Longrightarrow> sinvar \<lparr> nodes = N, edges = E' \<rparr> nP )"
       unfolding sinvar_mono_def
       by metis
     have "\<And> G FF F. {(e1, e2). (e1, e2) \<in> edges G \<and> (e1, e2) \<notin> FF \<and> (e1, e2) \<notin> F} \<subseteq> {(e1, e2). (e1, e2) \<in> edges G \<and> (e1, e2) \<notin> FF} "
       by(rule Collect_mono) (simp)
-    from sinvarE[OF validG' this]
+    from sinvarE[OF wfG' this]
     show "is_offending_flows FF G nP \<Longrightarrow> is_offending_flows (FF \<union> F) G nP"
       by(simp add: is_offending_flows_def delete_edges_def)
   qed
 
   (*use this to show locale sinvar_mono*)
   lemma sinvar_mono_imp_sinvar_mono: 
-  "sinvar_mono \<Longrightarrow> valid_graph \<lparr> nodes = N, edges = E \<rparr> \<Longrightarrow> E' \<subseteq> E \<Longrightarrow> sinvar \<lparr> nodes = N, edges = E \<rparr> nP \<Longrightarrow> 
+  "sinvar_mono \<Longrightarrow> wf_graph \<lparr> nodes = N, edges = E \<rparr> \<Longrightarrow> E' \<subseteq> E \<Longrightarrow> sinvar \<lparr> nodes = N, edges = E \<rparr> nP \<Longrightarrow> 
         sinvar \<lparr> nodes = N, edges = E' \<rparr> nP"
   apply(simp add: sinvar_mono_def)
   by blast
@@ -159,7 +159,7 @@ begin
 
 
 
-  (*lemma offending_min_set_ab_in_fs: "valid_graph (G::'v graph) \<Longrightarrow> (a,b) \<in> edges G \<Longrightarrow>
+  (*lemma offending_min_set_ab_in_fs: "wf_graph (G::'v graph) \<Longrightarrow> (a,b) \<in> edges G \<Longrightarrow>
        is_offending_flows_min_set ({(a, b)} \<union> fs) G nP \<Longrightarrow>
        sinvar (delete_edges G fs) nP \<Longrightarrow>
        (a,b) \<in> fs"
@@ -190,14 +190,14 @@ begin
 
   lemma not_model_mono_imp_addedge_mono: 
   assumes mono: "sinvar_mono"
-   and vG: "valid_graph G" and ain: "(a1,a2) \<in> edges G" and xy: "X \<subseteq> Y" and ns: "\<not> sinvar (add_edge a1 a2 (delete_edges G (Y))) nP"  
+   and vG: "wf_graph G" and ain: "(a1,a2) \<in> edges G" and xy: "X \<subseteq> Y" and ns: "\<not> sinvar (add_edge a1 a2 (delete_edges G (Y))) nP"  
   shows "\<not> sinvar (add_edge a1 a2 (delete_edges G X)) nP"
    proof -
-      have valid_graph_add_delete_edge_simp: 
+      have wf_graph_add_delete_edge_simp: 
         "\<And>Y. add_edge a1 a2 (delete_edges G Y) = (delete_edges G (Y - {(a1,a2)}))"
         apply(simp add: delete_edges_simp2 add_edge_def)
         apply(rule conjI)
-         using ain apply (metis insert_absorb vG valid_graph.E_validD(1) valid_graph.E_validD(2))
+         using ain apply (metis insert_absorb vG wf_graph.E_wfD(1) wf_graph.E_wfD(2))
          apply(auto simp add: ain)
         done
       from this ns have 1: "\<not> sinvar (delete_edges G (Y - {(a1, a2)})) nP" by simp
@@ -205,13 +205,13 @@ begin
       from sinvar_mono_imp_negative_delete_edge_mono[OF mono] vG have
         "\<And>X Y. X \<subseteq> Y \<Longrightarrow> \<not> sinvar (delete_edges G Y) nP \<Longrightarrow> \<not> sinvar (delete_edges G X) nP" by blast
       from this[OF 2 1] have "\<not> sinvar (delete_edges G (X - {(a1, a2)})) nP" by simp
-      from this valid_graph_add_delete_edge_simp[symmetric] show ?thesis by simp
+      from this wf_graph_add_delete_edge_simp[symmetric] show ?thesis by simp
    qed
 
 
   theorem is_offending_flows_min_set_minimalize_offending_overapprox:
       assumes mono: "sinvar_mono"
-      and vG: "valid_graph G" and iO: "is_offending_flows (set ff) G nP" and sF: "set ff \<subseteq> edges G" and dF: "distinct ff"
+      and vG: "wf_graph G" and iO: "is_offending_flows (set ff) G nP" and sF: "set ff \<subseteq> edges G" and dF: "distinct ff"
       shows "is_offending_flows_min_set (set (minimalize_offending_overapprox ff [] G nP)) G nP" (is "is_offending_flows_min_set ?minset G nP")
   proof -
     from iO have "sinvar (delete_edges G (set ff)) nP" by (metis is_offending_flows_def)
@@ -291,9 +291,9 @@ begin
                   apply(simp add:delete_edges_list_union delete_edges_list_union_insert)
                   apply(simp add: graph_ops)
                   apply(rule conjI)
-                   apply(simp add: valid_graph_def)
+                   apply(simp add: wf_graph_def)
                    apply blast
-                  apply(simp add: valid_graph_def)
+                  apply(simp add: wf_graph_def)
                   by fastforce
                 } note delete_edges_list_add_add_iff=this
                 from aE have "(fst a, snd a) \<in> edges G" by simp
@@ -343,13 +343,13 @@ begin
 
   corollary mono_imp_set_offending_flows_not_empty:
   assumes mono_sinvar: "sinvar_mono"
-  and vG: "valid_graph G" and iO: "is_offending_flows (set ff) G nP" and sS: "set ff \<subseteq> edges G" and dF: "distinct ff"
+  and vG: "wf_graph G" and iO: "is_offending_flows (set ff) G nP" and sS: "set ff \<subseteq> edges G" and dF: "distinct ff"
   shows
     "set_offending_flows G nP \<noteq> {}"
   proof -
     from iO SecurityInvariant_withOffendingFlows.is_offending_flows_def have nS: "\<not> sinvar G nP" by metis
     from sinvar_mono_imp_negative_delete_edge_mono[OF mono_sinvar] have negative_delete_edge_mono: 
-      "\<forall> G nP X Y. valid_graph G \<and> X \<subseteq> Y \<and> \<not> sinvar (delete_edges G (Y)) nP \<longrightarrow> \<not> sinvar (delete_edges G X) nP" by blast
+      "\<forall> G nP X Y. wf_graph G \<and> X \<subseteq> Y \<and> \<not> sinvar (delete_edges G (Y)) nP \<longrightarrow> \<not> sinvar (delete_edges G X) nP" by blast
       
     from is_offending_flows_min_set_minimalize_offending_overapprox[OF mono_sinvar vG iO sS dF] 
      have "is_offending_flows_min_set (set (minimalize_offending_overapprox ff [] G nP)) G nP" by simp
@@ -372,12 +372,12 @@ begin
    there a means to fix it if and only if the network in which nobody communicates with anyone fulfills the security requirement
    *}
    theorem valid_empty_edges_iff_exists_offending_flows: 
-    assumes mono: "sinvar_mono" and validG: "valid_graph G" and noteval: "\<not> sinvar G nP"
+    assumes mono: "sinvar_mono" and wfG: "wf_graph G" and noteval: "\<not> sinvar G nP"
     shows "sinvar \<lparr> nodes = nodes G, edges = {} \<rparr> nP \<longleftrightarrow> set_offending_flows G nP \<noteq> {}"
    proof 
       assume a: "sinvar \<lparr> nodes = nodes G, edges = {} \<rparr> nP"
   
-      from finite_distinct_list[OF valid_graph.finiteE] validG
+      from finite_distinct_list[OF wf_graph.finiteE] wfG
       obtain list_edges where list_edges_props: "set list_edges = edges G \<and> distinct list_edges" by blast
       hence listedges_subseteq_edges: "set list_edges \<subseteq> edges G" by blast
   
@@ -385,7 +385,7 @@ begin
       from a is_offending_flows_def noteval list_edges_props empty_edge_graph_simp 
         have overapprox: "is_offending_flows (set list_edges) G nP" by auto
   
-      from mono_imp_set_offending_flows_not_empty[OF mono validG overapprox listedges_subseteq_edges] list_edges_props 
+      from mono_imp_set_offending_flows_not_empty[OF mono wfG overapprox listedges_subseteq_edges] list_edges_props 
       show "set_offending_flows G nP \<noteq> {}" by simp
     next
       assume a: "set_offending_flows G nP \<noteq> {}"
@@ -394,11 +394,11 @@ begin
   
       from f_props have "sinvar (delete_edges G f) nP" using is_offending_flows_min_set_def is_offending_flows_def by simp
         hence evalGf: "sinvar \<lparr>nodes = nodes G, edges = {(e1, e2). (e1, e2) \<in> edges G \<and> (e1, e2) \<notin> f}\<rparr> nP" by(simp add: delete_edges_def)
-      from delete_edges_valid[OF validG, unfolded delete_edges_def] 
-        have validGf: "valid_graph \<lparr>nodes = nodes G, edges = {(e1, e2). (e1, e2) \<in> edges G \<and> (e1, e2) \<notin> f}\<rparr>" by simp
+      from delete_edges_wf[OF wfG, unfolded delete_edges_def] 
+        have wfGf: "wf_graph \<lparr>nodes = nodes G, edges = {(e1, e2). (e1, e2) \<in> edges G \<and> (e1, e2) \<notin> f}\<rparr>" by simp
       have emptyseqGf: "{} \<subseteq>  {(e1, e2). (e1, e2) \<in> edges G \<and> (e1, e2) \<notin> f}" by simp
   
-      from mono[unfolded sinvar_mono_def] evalGf validGf emptyseqGf have "sinvar \<lparr>nodes = nodes G, edges = {}\<rparr> nP" by blast
+      from mono[unfolded sinvar_mono_def] evalGf wfGf emptyseqGf have "sinvar \<lparr>nodes = nodes G, edges = {}\<rparr> nP" by blast
       thus "sinvar \<lparr>nodes = nodes G, edges = {}\<rparr> nP" .
   qed
 
@@ -430,22 +430,22 @@ context SecurityInvariant_preliminaries
       unfolding sinvar_mono_def using mono_sinvar by blast
 
     text{*Note: due to monotonicity, the minimality also holds for arbitrary subsets *}
-    lemma assumes "valid_graph G" and "is_offending_flows_min_set F G nP" and "F \<subseteq> edges G" and "E \<subseteq> F" and "E \<noteq> {}"
+    lemma assumes "wf_graph G" and "is_offending_flows_min_set F G nP" and "F \<subseteq> edges G" and "E \<subseteq> F" and "E \<noteq> {}"
           shows "\<not> sinvar \<lparr> nodes = nodes G, edges = ((edges G) - F) \<union> E \<rparr> nP"
     proof -
-      from sinvar_mono_imp_negative_delete_edge_mono[OF sinvar_monoI `valid_graph G`] have negative_delete_edge_mono: 
+      from sinvar_mono_imp_negative_delete_edge_mono[OF sinvar_monoI `wf_graph G`] have negative_delete_edge_mono: 
       "\<And>X Y. X \<subseteq> Y \<Longrightarrow> \<not> sinvar \<lparr> nodes = nodes G, edges = (edges G) - Y \<rparr> nP \<Longrightarrow> \<not> sinvar \<lparr> nodes = nodes G, edges = edges G - X \<rparr> nP"
         using delete_edges_simp2 by metis
       from assms(2) have "(\<forall>(e1, e2)\<in>F. \<not> sinvar (add_edge e1 e2 (delete_edges G F)) nP)"
       unfolding is_offending_flows_min_set_def by simp
-      with `valid_graph G` have min: "(\<forall>(e1, e2)\<in>F. \<not> sinvar \<lparr> nodes = nodes G, edges = ((edges G) - F) \<union> {(e1,e2)} \<rparr> nP)"
+      with `wf_graph G` have min: "(\<forall>(e1, e2)\<in>F. \<not> sinvar \<lparr> nodes = nodes G, edges = ((edges G) - F) \<union> {(e1,e2)} \<rparr> nP)"
         apply(simp add: delete_edges_simp2 add_edge_def)
         apply(rule, rename_tac x, case_tac x, rename_tac e1 e2, simp)
         apply(erule_tac x="(e1, e2)" in ballE)
          apply(simp_all)
         apply(subgoal_tac "insert e1 (insert e2 (nodes G)) = nodes G")
          apply(simp)
-        by (metis assms(3) insert_absorb set_rev_mp valid_graph.E_validD(1) valid_graph.E_validD(2))
+        by (metis assms(3) insert_absorb set_rev_mp wf_graph.E_wfD(1) wf_graph.E_wfD(2))
       from `E \<noteq> {}` obtain e where "e \<in> E" by blast
       with min `E \<subseteq> F` have mine: "\<not> sinvar \<lparr> nodes = nodes G, edges = ((edges G) - F) \<union> {e} \<rparr> nP" by fast
       have e1: "edges G - (F - {e}) = insert e (edges G - F)" using DiffD2 `e \<in> E` assms(3) assms(4) by auto 
@@ -458,7 +458,7 @@ context SecurityInvariant_preliminaries
     
     text{* The algorithm @{const minimalize_offending_overapprox} is correct *}
     lemma minimalize_offending_overapprox_sound: 
-      "\<lbrakk> valid_graph G; is_offending_flows (set ff) G nP; set ff \<subseteq> edges G; distinct ff \<rbrakk>
+      "\<lbrakk> wf_graph G; is_offending_flows (set ff) G nP; set ff \<subseteq> edges G; distinct ff \<rbrakk>
         \<Longrightarrow> is_offending_flows_min_set (set (minimalize_offending_overapprox ff [] G nP)) G nP "
     using is_offending_flows_min_set_minimalize_offending_overapprox sinvar_monoI by blast
 
@@ -470,7 +470,7 @@ context SecurityInvariant_preliminaries
       Note: choosing ff = edges G is a good choice!
     *}
     theorem minimalize_offending_overapprox_gives_back_an_offending_flow:
-      "\<lbrakk> valid_graph G; is_offending_flows (set ff) G nP; set ff \<subseteq> edges G; distinct ff \<rbrakk>
+      "\<lbrakk> wf_graph G; is_offending_flows (set ff) G nP; set ff \<subseteq> edges G; distinct ff \<rbrakk>
         \<Longrightarrow>
          (set (minimalize_offending_overapprox ff [] G nP)) \<in> set_offending_flows G nP"
     apply(frule(3) minimalize_offending_overapprox_sound)
@@ -480,7 +480,7 @@ context SecurityInvariant_preliminaries
 
     (*TODO better minimality condition for keeps*)
     (*lemma  minimalize_offending_overapprox_sound_fixKeep:
-      "\<lbrakk> valid_graph G; is_offending_flows (set (ff @ keeps)) G nP; \<forall> x \<in> set ff. x \<notin> set keeps; \<forall> x \<in> set ff. x \<in> edges G; distinct ff; 
+      "\<lbrakk> wf_graph G; is_offending_flows (set (ff @ keeps)) G nP; \<forall> x \<in> set ff. x \<notin> set keeps; \<forall> x \<in> set ff. x \<in> edges G; distinct ff; 
         \<forall>(e1, e2)\<in> set keeps. \<not> sinvar (add_edge e1 e2 (delete_edges G (set (minimalize_offending_overapprox ff keeps G nP)))) nP \<rbrakk>
         \<Longrightarrow>
          is_offending_flows_min_set (set (minimalize_offending_overapprox ff keeps G nP)) G nP \<and> set keeps \<subseteq> (set (minimalize_offending_overapprox ff keeps G nP))"
@@ -512,15 +512,15 @@ begin
     text{*If there is a violation and there are no offending flows, there does not exist a possibility to fix the violation by 
           tightening the policy. @{thm valid_empty_edges_iff_exists_offending_flows} already hints this. *}
     lemma mono_imp_emptyoffending_eq_nevervalid:
-       "\<lbrakk> sinvar_mono; valid_graph G; \<not> sinvar G nP; set_offending_flows G nP = {}\<rbrakk> \<Longrightarrow> 
+       "\<lbrakk> sinvar_mono; wf_graph G; \<not> sinvar G nP; set_offending_flows G nP = {}\<rbrakk> \<Longrightarrow> 
         \<not> (\<exists> F \<subseteq> edges G. sinvar (delete_edges G F) nP)"
     proof -
       assume mono: "sinvar_mono"
-      and validG: "valid_graph G"
+      and wfG: "wf_graph G"
       and a1:  "\<not> sinvar G nP"
       and a2: "set_offending_flows G nP = {}"
 
-      from validG have validG': "valid_graph \<lparr>nodes = nodes G, edges = edges G\<rparr>" by(simp add:valid_graph_def)
+      from wfG have wfG': "wf_graph \<lparr>nodes = nodes G, edges = edges G\<rparr>" by(simp add:wf_graph_def)
 
       from a2 set_offending_flows_def have "\<forall>f \<subseteq> edges G. \<not> is_offending_flows_min_set f G nP" by simp
       from this is_offending_flows_min_set_def is_offending_flows_def a1 have notdeleteconj:
@@ -543,18 +543,18 @@ begin
             hence "\<exists>(e1,e2)\<in>f. sinvar (add_edge e1 e2 (delete_edges G f)) nP" by(auto)
             from this obtain e1 e2 where e1e2cond: "(e1,e2)\<in>f \<and> sinvar (add_edge e1 e2 (delete_edges G f)) nP" by blast
             
-            from `f \<subseteq> edges G` validG have "finite f" apply(simp add: valid_graph_def) by (metis rev_finite_subset)
+            from `f \<subseteq> edges G` wfG have "finite f" apply(simp add: wf_graph_def) by (metis rev_finite_subset)
             from this obtain listf where listf: "set listf = f \<and> distinct listf" by (metis finite_distinct_list)
 
             from e1e2cond `f \<subseteq> edges G` have Geq:
             "(add_edge e1 e2 (delete_edges G f)) = \<lparr> nodes = nodes G, edges = edges G - f \<union> {(e1,e2)}\<rparr>"
-              apply(simp add: graph_ops validG')
+              apply(simp add: graph_ops wfG')
               apply(clarify)
-               using validG[unfolded valid_graph_def] by force
+               using wfG[unfolded wf_graph_def] by force
 
 
-            from this[symmetric] add_edge_valid[OF delete_edges_valid[OF validG]] have 
-              "valid_graph \<lparr>nodes = nodes G, edges = edges G - f \<union> {(e1, e2)}\<rparr>" by simp
+            from this[symmetric] add_edge_wf[OF delete_edges_wf[OF wfG]] have 
+              "wf_graph \<lparr>nodes = nodes G, edges = edges G - f \<union> {(e1, e2)}\<rparr>" by simp
             from mono this  have mono'':
               "\<And> E'. E' \<subseteq> edges G - f \<union> {(e1, e2)} \<Longrightarrow>
                 sinvar \<lparr>nodes = nodes G, edges = edges G - f \<union> {(e1, e2)}\<rparr> nP \<Longrightarrow> 
@@ -569,7 +569,7 @@ begin
             from this listf have c1: "is_offending_flows (set listf) G nP" by(simp add: is_offending_flows_def)
             from listf `f \<subseteq> edges G` have c2: "set listf \<subseteq> edges G" by simp
 
-            from mono_imp_set_offending_flows_not_empty[OF mono validG c1 c2 conjunct2[OF listf]] have 
+            from mono_imp_set_offending_flows_not_empty[OF mono wfG c1 c2 conjunct2[OF listf]] have 
               "set_offending_flows G nP \<noteq> {}" .
             from this a2 have "False" by simp
             (*I knew this can't be!*)
@@ -588,7 +588,7 @@ text{* Old version of security invariant gave @{term "F \<in> set_offending_flow
 context SecurityInvariant_withOffendingFlows
 begin
   lemma mono_exists_offending_flows:
-  "\<lbrakk> sinvar_mono; valid_graph G; is_offending_flows (set ff) G nP; set ff \<subseteq> edges G; distinct ff \<rbrakk> 
+  "\<lbrakk> sinvar_mono; wf_graph G; is_offending_flows (set ff) G nP; set ff \<subseteq> edges G; distinct ff \<rbrakk> 
     \<Longrightarrow> \<exists>F. F \<in> set_offending_flows G nP \<and> sinvar (delete_edges G F) nP"
     apply(frule mono_imp_set_offending_flows_not_empty[of G nP ff])
          apply(simp_all add:is_offending_flows_def)
@@ -615,10 +615,10 @@ subsection {* Monotonicity of offending flows *}
     text{*If there is some @{term "F'"} in the offending flows of a small graph and you have a bigger graph, 
           you can extend @{term "F'"} by some @{term "Fadd"} and minimality in @{term F} is preserved *}
     lemma minimality_offending_flows_mono_edges_graph_extend:
-    "\<lbrakk> valid_graph \<lparr> nodes = V, edges = E \<rparr>; E' \<subseteq> E; Fadd \<inter> E' = {}; F' \<in> set_offending_flows \<lparr>nodes = V, edges = E'\<rparr> nP \<rbrakk> \<Longrightarrow> 
+    "\<lbrakk> wf_graph \<lparr> nodes = V, edges = E \<rparr>; E' \<subseteq> E; Fadd \<inter> E' = {}; F' \<in> set_offending_flows \<lparr>nodes = V, edges = E'\<rparr> nP \<rbrakk> \<Longrightarrow> 
             (\<forall>(e1, e2)\<in>F'. \<not> sinvar (add_edge e1 e2 (delete_edges \<lparr>nodes = V, edges = E \<rparr> (F' \<union> Fadd))) nP)"
     proof -
-      assume a1: "valid_graph \<lparr> nodes = V, edges = E \<rparr>"
+      assume a1: "wf_graph \<lparr> nodes = V, edges = E \<rparr>"
       and    a2: "E' \<subseteq> E"
       and    a3: "Fadd \<inter> E' = {}"
       and    a4: "F' \<in> set_offending_flows \<lparr>nodes = V, edges = E'\<rparr> nP"
@@ -628,7 +628,7 @@ subsection {* Monotonicity of offending flows *}
       obtain Eadd where Eadd_prop: "E' \<union> Eadd = E" and "E' \<inter> Eadd = {}" using a2 by blast
 
       have Fadd_notinE': "\<And>Fadd. Fadd \<inter> E' = {} \<Longrightarrow>  E' - (F' \<union> Fadd) =  E' - F'" by blast
-      from `F' \<subseteq> E'` a1[simplified valid_graph_def] a2 have FinV1: "fst ` F' \<subseteq> V" and FinV2: "snd ` F' \<subseteq> V" 
+      from `F' \<subseteq> E'` a1[simplified wf_graph_def] a2 have FinV1: "fst ` F' \<subseteq> V" and FinV2: "snd ` F' \<subseteq> V" 
           apply (simp_all)
          apply(erule conjE)+
          apply(drule image_mono[of _ _ "fst"])+
@@ -677,8 +677,8 @@ subsection {* Monotonicity of offending flows *}
               from this[OF f1] f2 have gFadd1: "\<not> sinvar \<lparr>nodes = V, edges = (E' - (F' \<union> Fadd)) \<union> {(e1, e2)}\<rparr> nP" by simp
        
               from a1 FinV1 FinV2 f1 f2 have gFadd2: 
-                  "valid_graph \<lparr>nodes = V, edges = (E - (F' \<union> Fadd)) \<union> {(e1, e2)}\<rparr>"
-                  by(auto simp add: valid_graph_def)
+                  "wf_graph \<lparr>nodes = V, edges = (E - (F' \<union> Fadd)) \<union> {(e1, e2)}\<rparr>"
+                  by(auto simp add: wf_graph_def)
        
               from a2 f1 f2 have gFadd3: 
                    "(E' - (F' \<union> Fadd)) \<union> {(e1, e2)} \<subseteq> (E - (F' \<union> Fadd)) \<union> {(e1, e2)}" by fast
@@ -698,7 +698,7 @@ subsection {* Monotonicity of offending flows *}
 
     text{* The minimality condition of the offending flows also holds if we increase the graph.  *}
     corollary minimality_offending_flows_mono_edges_graph: 
-      "\<lbrakk> valid_graph \<lparr> nodes = V, edges = E \<rparr>; 
+      "\<lbrakk> wf_graph \<lparr> nodes = V, edges = E \<rparr>; 
          E' \<subseteq> E;
          F \<in> set_offending_flows \<lparr>nodes = V, edges = E'\<rparr> nP \<rbrakk> \<Longrightarrow>
       \<forall>(e1, e2)\<in>F. \<not> sinvar (add_edge e1 e2 (delete_edges \<lparr>nodes = V, edges = E \<rparr> F)) nP"
@@ -706,26 +706,26 @@ subsection {* Monotonicity of offending flows *}
 
 
     text{* all sets in the set of offending flows are monotonic, hence, for a larger graph, they can be extended to match the smaller graph. I.e. everything is monotonic. *}
-    theorem mono_extend_set_offending_flows: "\<lbrakk> valid_graph \<lparr> nodes = V, edges = E \<rparr>; E' \<subseteq> E; F' \<in> set_offending_flows \<lparr> nodes = V, edges = E' \<rparr> nP \<rbrakk> \<Longrightarrow>
+    theorem mono_extend_set_offending_flows: "\<lbrakk> wf_graph \<lparr> nodes = V, edges = E \<rparr>; E' \<subseteq> E; F' \<in> set_offending_flows \<lparr> nodes = V, edges = E' \<rparr> nP \<rbrakk> \<Longrightarrow>
         \<exists> F \<in> set_offending_flows \<lparr> nodes = V, edges = E \<rparr> nP. F' \<subseteq> F"
       proof -
         fix F'V E E'
-        assume a1: "valid_graph \<lparr> nodes = V, edges = E \<rparr>"
+        assume a1: "wf_graph \<lparr> nodes = V, edges = E \<rparr>"
         and    a2: "E' \<subseteq> E"
         and    a4: "F' \<in> set_offending_flows \<lparr>nodes = V, edges = E'\<rparr> nP"
 
         --{* Idea: @{text "F = F' \<union> minimize (E - E')"}*}
   
-        have "\<And>f. valid_graph (delete_edges \<lparr>nodes = V, edges = E\<rparr> f)"
-        using delete_edges_valid[OF a1] by fast
-        hence valid1: "\<And>f. valid_graph \<lparr>nodes = V, edges = E -f\<rparr>"
+        have "\<And>f. wf_graph (delete_edges \<lparr>nodes = V, edges = E\<rparr> f)"
+        using delete_edges_wf[OF a1] by fast
+        hence wf1: "\<And>f. wf_graph \<lparr>nodes = V, edges = E -f\<rparr>"
         by(simp add: delete_edges_simp2)
   
         obtain Eadd where Eadd_prop: "E' \<union> Eadd = E" and "E' \<inter> Eadd = {}" using a2 by blast
   
         from a4 have "F' \<subseteq> E'" by(simp add: set_offending_flows_def)
   
-        from valid1 have valid2: "valid_graph \<lparr>nodes = V, edges = E' - F' \<union> Eadd\<rparr>"
+        from wf1 have wf2: "wf_graph \<lparr>nodes = V, edges = E' - F' \<union> Eadd\<rparr>"
           apply(subgoal_tac "E' - F' \<union> Eadd = E - F'")
            apply fastforce
           using Eadd_prop `E' \<inter> Eadd = {}` `F' \<subseteq> E'` by fast
@@ -750,11 +750,11 @@ subsection {* Monotonicity of offending flows *}
         proof(cases "\<not> sinvar \<lparr>nodes = V, edges = E' - F' \<union> Eadd\<rparr> nP")
           assume assumption_new_violation: "\<not> sinvar \<lparr>nodes = V, edges = E' - F' \<union> Eadd\<rparr> nP"
           from a1 have "finite Eadd"
-            apply(simp add: valid_graph_def)
+            apply(simp add: wf_graph_def)
             using Eadd_prop by (metis finite_Un)
           from this obtain Eadd_list where Eadd_list_prop: "set Eadd_list = Eadd" and "distinct Eadd_list" by (metis finite_distinct_list)
           from a1 have "finite E'"
-            apply(simp add: valid_graph_def)
+            apply(simp add: wf_graph_def)
             using Eadd_prop by (metis finite_Un)
           from this obtain E'_list where E'_list_prop: "set E'_list = E'" and "distinct E'_list" by (metis finite_distinct_list)
           from `finite E'` `F' \<subseteq> E'` obtain F'_list where "set F'_list = F'" and "distinct F'_list" by (metis finite_distinct_list rev_finite_subset)
@@ -769,7 +769,7 @@ subsection {* Monotonicity of offending flows *}
             done
         
         
-          from minimalize_offending_overapprox_sound[OF valid2 this _ `distinct Eadd_list`]
+          from minimalize_offending_overapprox_sound[OF wf2 this _ `distinct Eadd_list`]
           have "is_offending_flows_min_set (set (minimalize_offending_overapprox Eadd_list [] \<lparr>nodes = V, edges = E' - F' \<union> Eadd\<rparr> nP)) \<lparr>nodes = V, edges = E' - F' \<union> Eadd\<rparr> nP"
           by(simp add: Eadd_list_prop)
         
@@ -848,7 +848,7 @@ subsection {* Monotonicity of offending flows *}
 
 
     text{* The offending flows are monotonic. *}
-    corollary offending_flows_union_mono: "\<lbrakk> valid_graph \<lparr> nodes = V, edges = E \<rparr>; E' \<subseteq> E \<rbrakk> \<Longrightarrow> 
+    corollary offending_flows_union_mono: "\<lbrakk> wf_graph \<lparr> nodes = V, edges = E \<rparr>; E' \<subseteq> E \<rbrakk> \<Longrightarrow> 
       (\<Union> set_offending_flows \<lparr> nodes = V, edges = E' \<rparr> nP) \<subseteq> (\<Union> set_offending_flows \<lparr> nodes = V, edges = E \<rparr> nP)"
       apply(clarify)
       apply(drule(2) mono_extend_set_offending_flows)
@@ -857,14 +857,14 @@ subsection {* Monotonicity of offending flows *}
 
 
    (* I guess set_offending_flows = {{e}} does not hold. Consider the Dependability invariant:
-      having a valid graph.
+      having a wf graph.
       Add an edge s.t. a dependability violation occurs.
       The offending flows now contains the new edge ans all edges on the path from the node with the violation to the end of the new edge. *)
    lemma set_offending_flows_insert_contains_new:
-   "\<lbrakk> valid_graph \<lparr> nodes = V, edges = insert e E \<rparr>; set_offending_flows \<lparr>nodes = V, edges = E\<rparr> nP = {}; set_offending_flows \<lparr>nodes = V, edges = insert e E\<rparr> nP \<noteq> {} \<rbrakk> \<Longrightarrow> 
+   "\<lbrakk> wf_graph \<lparr> nodes = V, edges = insert e E \<rparr>; set_offending_flows \<lparr>nodes = V, edges = E\<rparr> nP = {}; set_offending_flows \<lparr>nodes = V, edges = insert e E\<rparr> nP \<noteq> {} \<rbrakk> \<Longrightarrow> 
       {e} \<in> set_offending_flows \<lparr>nodes = V, edges = insert e E\<rparr> nP"
      proof -
-       assume validG: "valid_graph \<lparr> nodes = V, edges = insert e E \<rparr>"
+       assume wfG: "wf_graph \<lparr> nodes = V, edges = insert e E \<rparr>"
        and    a1: "set_offending_flows \<lparr>nodes = V, edges = E\<rparr> nP = {}"
        and    a2: "set_offending_flows \<lparr>nodes = V, edges = insert e E\<rparr> nP \<noteq> {}"
 
@@ -875,10 +875,10 @@ subsection {* Monotonicity of offending flows *}
        from a2 have a2': "\<exists>F \<subseteq> insert e E. is_offending_flows_min_set F \<lparr>nodes = V, edges = insert e E\<rparr> nP"
         by(simp add: set_offending_flows_def)
 
-       from validG have validG': "valid_graph \<lparr> nodes = V, edges = E \<rparr>" by(simp add:valid_graph_def)
+       from wfG have wfG': "wf_graph \<lparr> nodes = V, edges = E \<rparr>" by(simp add:wf_graph_def)
 
-       from a1 defined_offending[OF validG'] have evalG: "sinvar \<lparr>nodes = V, edges = E \<rparr> nP" by blast
-       from sinvar_monoI[unfolded sinvar_mono_def] validG' this
+       from a1 defined_offending[OF wfG'] have evalG: "sinvar \<lparr>nodes = V, edges = E \<rparr> nP" by blast
+       from sinvar_monoI[unfolded sinvar_mono_def] wfG' this
        have goal_eval: "sinvar \<lparr>nodes = V, edges = E - {e}\<rparr> nP" by (metis Diff_subset)
 
        from sinvar_no_offending a2 have goal_not_eval: "\<not> sinvar \<lparr>nodes = V, edges = insert e E\<rparr> nP" by blast
@@ -896,8 +896,8 @@ subsection {* Monotonicity of offending flows *}
          using goal_not_eval apply fastforce
         apply(thin_tac "\<forall>F \<subseteq> E. X F" for X)
         apply(thin_tac "\<exists>F \<subseteq> E. X F" for E X)
-        apply(insert validG)
-        apply(simp add: valid_graph_def)
+        apply(insert wfG)
+        apply(simp add: wf_graph_def)
         apply(fastforce)
         done
 
@@ -970,14 +970,14 @@ end
 
     lemma offending_partition_subset_empty: 
     assumes a1:"\<forall> F \<in> (set_offending_flows \<lparr>nodes = V, edges = E \<union> X\<rparr> nP). F \<subseteq> X"
-    and validGEX: "valid_graph \<lparr>nodes = V, edges = E \<union> X\<rparr>"
+    and wfGEX: "wf_graph \<lparr>nodes = V, edges = E \<union> X\<rparr>"
     and disj: "E \<inter> X = {}"
     shows "(set_offending_flows \<lparr>nodes = V, edges = E\<rparr> nP) = {}"
     proof(rule ccontr)
       assume c: "set_offending_flows \<lparr>nodes = V, edges = E\<rparr> nP \<noteq> {}"
       from this obtain F' where F'_prop: "F' \<in> set_offending_flows \<lparr>nodes = V, edges = E\<rparr> nP" by blast
       from F'_prop have "F' \<subseteq> E" using set_offending_flows_def by simp
-      from mono_extend_set_offending_flows[OF validGEX _ F'_prop] have 
+      from mono_extend_set_offending_flows[OF wfGEX _ F'_prop] have 
         "\<exists>F\<in>set_offending_flows \<lparr>nodes = V, edges = E \<union> X\<rparr> nP. F' \<subseteq> F" by blast
       from this a1 have "F' \<subseteq> X" by fast
       from F'_prop have "{} \<noteq> F'" by (metis empty_offending_contra)
@@ -986,11 +986,11 @@ end
     qed
 
     corollary partitioned_offending_subseteq_pow_combine:
-    assumes validGEX: "valid_graph \<lparr>nodes = V, edges = E \<union> X\<rparr>"
+    assumes wfGEX: "wf_graph \<lparr>nodes = V, edges = E \<union> X\<rparr>"
     and disj: "E \<inter> X = {}"
     and partitioned_offending: "\<forall> F \<in> (set_offending_flows \<lparr>nodes = V, edges = E \<union> X\<rparr> nP). F \<subseteq> X" (*offending does not contain E*)
     shows "(set_offending_flows \<lparr>nodes = V, edges = E \<union> X\<rparr> nP) \<subseteq> pow_combine X (set_offending_flows \<lparr>nodes = V, edges = E\<rparr> nP)"
-    apply(subst offending_partition_subset_empty[OF partitioned_offending validGEX disj])
+    apply(subst offending_partition_subset_empty[OF partitioned_offending wfGEX disj])
     apply(simp add: pow_combine_def)
     apply(rule)
     apply(simp)
@@ -1004,18 +1004,18 @@ end
     text{* Knowing that the @{text "\<Union> offending is \<subseteq> X"}, removing something from the graphs's edges, 
            it also disappears from the offending flows. *}
     lemma Un_set_offending_flows_bound_minus:
-    assumes validG: "valid_graph \<lparr> nodes = V, edges = E \<rparr>"
+    assumes wfG: "wf_graph \<lparr> nodes = V, edges = E \<rparr>"
     and     Foffending: "\<Union> set_offending_flows \<lparr>nodes = V, edges = E\<rparr> nP \<subseteq> X"
     shows   "\<Union> set_offending_flows \<lparr>nodes = V, edges = E - {f}\<rparr> nP \<subseteq> X - {f}"
     proof -
-      from validG have validG': "valid_graph \<lparr> nodes = V, edges = E - {f} \<rparr>"
-        by(auto simp add: valid_graph_def finite_subset)
+      from wfG have wfG': "wf_graph \<lparr> nodes = V, edges = E - {f} \<rparr>"
+        by(auto simp add: wf_graph_def finite_subset)
       
-      from offending_flows_union_mono[OF validG, where E'="E - {f}"] have 
+      from offending_flows_union_mono[OF wfG, where E'="E - {f}"] have 
         "\<Union>set_offending_flows \<lparr>nodes = V, edges = E - {f}\<rparr> nP - {f} \<subseteq> \<Union>set_offending_flows \<lparr>nodes = V, edges = E\<rparr> nP - {f}" by blast
       also have 
         "\<Union>set_offending_flows \<lparr>nodes = V, edges = E - {f}\<rparr> nP \<subseteq> \<Union>set_offending_flows \<lparr>nodes = V, edges = E - {f}\<rparr> nP - {f}"
-        apply(simp add: set_offending_flows_simp[OF validG']) by blast
+        apply(simp add: set_offending_flows_simp[OF wfG']) by blast
       ultimately have Un_set_offending_flows_minus:
         "\<Union> set_offending_flows \<lparr>nodes = V, edges = E - {f}\<rparr> nP \<subseteq> \<Union> set_offending_flows \<lparr>nodes = V, edges = E \<rparr> nP - {f}"
         by blast
@@ -1031,18 +1031,18 @@ end
     and the offending flows from the smaller graph are bound by @{term "X - E'"}.
   *}
     lemma Un_set_offending_flows_bound_minus_subseteq:
-    assumes validG: "valid_graph \<lparr> nodes = V, edges = E \<rparr>"
+    assumes wfG: "wf_graph \<lparr> nodes = V, edges = E \<rparr>"
     and     Foffending: "\<Union> set_offending_flows \<lparr>nodes = V, edges = E\<rparr> nP \<subseteq> X"
     shows   "\<Union> set_offending_flows \<lparr>nodes = V, edges = E - E'\<rparr> nP \<subseteq> X - E'"
     proof -
-      from validG have validG': "valid_graph \<lparr> nodes = V, edges = E - E' \<rparr>"
-        by(auto simp add: valid_graph_def finite_subset)
+      from wfG have wfG': "wf_graph \<lparr> nodes = V, edges = E - E' \<rparr>"
+        by(auto simp add: wf_graph_def finite_subset)
       
-      from offending_flows_union_mono[OF validG, where E'="E - E'"] have 
+      from offending_flows_union_mono[OF wfG, where E'="E - E'"] have 
         "(\<Union>set_offending_flows \<lparr>nodes = V, edges = E - E'\<rparr> nP) - E' \<subseteq> (\<Union>set_offending_flows \<lparr>nodes = V, edges = E\<rparr> nP) - E'" by blast
       also have 
         "\<Union>set_offending_flows \<lparr>nodes = V, edges = E - E'\<rparr> nP \<subseteq> \<Union>set_offending_flows \<lparr>nodes = V, edges = E - E'\<rparr> nP - E'"
-        apply(simp add: set_offending_flows_simp[OF validG']) by blast
+        apply(simp add: set_offending_flows_simp[OF wfG']) by blast
       ultimately have Un_set_offending_flows_minus:
         "\<Union> set_offending_flows \<lparr>nodes = V, edges = E - E'\<rparr> nP \<subseteq> \<Union> set_offending_flows \<lparr>nodes = V, edges = E \<rparr> nP - E'"
         by blast
@@ -1052,7 +1052,7 @@ end
     qed
 
   corollary Un_set_offending_flows_bound_minus_subseteq': 
-    "\<lbrakk> valid_graph \<lparr> nodes = V, edges = E \<rparr>;
+    "\<lbrakk> wf_graph \<lparr> nodes = V, edges = E \<rparr>;
     \<Union> set_offending_flows \<lparr> nodes = V, edges = E \<rparr> nP \<subseteq> X \<rbrakk> \<Longrightarrow>
     \<Union> set_offending_flows \<lparr> nodes = V, edges = E - E' \<rparr> nP \<subseteq> X - E'"
     apply(drule(1) Un_set_offending_flows_bound_minus_subseteq) by blast
