Network_Security_Policy_Verification/Examples/Distributed_WebApp.thy
@@ -18,7 +18,7 @@ definition policy :: "vString list_graph" where
                 edgesL = [] \<rparr>"
 
 text{*Sanity check*}
-lemma "valid_list_graph policy" by eval
+lemma "wf_list_graph policy" by eval
 (*proof by eval means we have executable code to show the lemma.*)
 
 
